theories/interop/wp_ext_call_laws.v
@@ -15,7 +15,7 @@ Context `{!wrapperG Σ}.
 Lemma base_prim_correct (p : prim) e Ψ :
   p ≠ Pcallback →
   (∀ e, p ≠ Pmain e) →
-  |- prims_prog e :: prim_proto p Ψ.
+  |- wrap_prog e :: prim_proto p Ψ.
 Proof using.
   intros Hncb Hnmain.
   (destruct p; try by congruence); unfold prim_proto.
